Schema changes

common-da-api/src/main/scala/de/qaware/findfacts/common/da/api/DocumentKind.scala
@@ -1,0 +1,19 @@
+package de.qaware.findfacts.common.da.api
+
+import enumeratum.EnumEntry
+
+import de.qaware.findfacts.common.utils.DefaultEnum
+
+/** Union type for doc kinds. */
+sealed trait DocumentKind extends EnumEntry
+
+/** Kind of documents */
+object DocumentKind extends DefaultEnum[DocumentKind] {
+  override final val values = findValues
+
+  /** Parent docs. */
+  case object Parent extends DocumentKind
+
+  /** Child docs. */
+  case object Child extends DocumentKind
+}
