search-core/src/it/scala/de/qaware/findfacts/core/SimpleQueryIT.scala
@@ -26,7 +26,15 @@ class SimpleQueryIT extends FunSuite with BeforeAndAfterAll with Matchers with I
       CodeblockEt("ExampleThy.1.11", "ExampleThy", 1, "fun", "\n", "fun Example = ...", "\n...", List(const1))
     val fact1 = FactEt("Fact.ExampleThy.ConstIsFact", "ConstIsFact", List(const1.id))
     val block2 =
-      CodeblockEt("ExampleThy.12.14", "ExampleThy", 3, "lemma", "\n...", "lemma ...", "(* stuff *)", List(fact1))
+      CodeblockEt(
+        "ExampleThy.12.14",
+        "ExampleThy",
+        3,
+        "lemma",
+        "\n...",
+        "lemma example_lem...",
+        "(* stuff *)",
+        List(fact1))
 
     val mapper = ToSolrDoc[BaseEt]
     itSolr.add(mapper.toSolrDoc(block1))
@@ -68,7 +76,7 @@ class SimpleQueryIT extends FunSuite with BeforeAndAfterAll with Matchers with I
   }
 
   test("Recursive query") {
-    val innerQuery = List(FieldFilter(EtField.Kind, Exact(Kind.Constant.toString)))
+    val innerQuery = List(FieldFilter(EtField.Kind, Exact(Kind.Constant.entryName)))
     val query = FilterQuery(List(FieldFilter(Uses, InResult(EtField.Id, innerQuery))))
     val result = queryModule.service.getResultShortlist(query)
 
@@ -83,5 +91,29 @@ class SimpleQueryIT extends FunSuite with BeforeAndAfterAll with Matchers with I
 
     val resultFacet = result.get
     resultFacet should equal(Map(EtField.StartLine -> Map("1" -> 1, "3" -> 1)))
+  }
+
+  test("Query with connectives") {
+    val query =
+      FilterQuery(List(FieldFilter(EtField.Kind, Not(Or(Exact(Kind.Fact.entryName), Exact(Kind.Type.entryName))))))
+    val result = queryModule.service.getResultShortlist(query)
+
+    val resList = result.get
+    resList.values should have size 1
+
+    val thyRes = resList.values.head.entities
+    thyRes should have size 1
+    thyRes.head.kind should equal(Kind.Constant)
+  }
+
+  test("Result scoring") {
+    val query = FilterQuery(List(FieldFilter(EtField.SourceText, Or(Exact("example"), Exact("lemma")))))
+    val result = queryModule.service.getResultShortlist(query)
+
+    val resList = result.get
+    resList.values should have size 2
+
+    val first = resList.values.head
+    first.command should equal("lemma")
   }
 }
