search-core/src/main/scala/de/qaware/findfacts/core/solrimpl/SolrQueryLiterals.scala
@@ -1,5 +1,6 @@
 package de.qaware.findfacts.core.solrimpl
 
+import de.qaware.findfacts.common.da.api.DocumentKind
 import de.qaware.findfacts.common.dt.Kind
 import de.qaware.findfacts.common.dt.solr.SolrSchema
 
@@ -13,13 +14,13 @@ object SolrQueryLiterals {
   final val OR = "||"
 
   /** Inverts a query or term. */
-  final val NOT = "!"
+  final val NOT = "* !"
 
   /** Term to get all. */
   final val ALL = "*"
 
   /** Query to filter parent values. */
-  final val QUERY_PARENT = s"${SolrSchema.DocKind}:${Kind.Block}"
+  final val QUERY_PARENT = s"${SolrSchema.DocKind}:${DocumentKind.Parent}"
 
   /** Query to get all values. */
   final val QUERY_ALL = s"$ALL:$ALL"
